# Basic methods for simpliifying function

## Definitoin:

### Combining Trems:

1. Theorem: XY + XY' = X

2. Example:

   1. abc'd' + abcd' = abd' 

      >  [X = abd', Y = c]

   2. ab'c + abc + a'bc = ac + bc

   3. (a + bc)(d + e') + a'(b'+c')(d + e') = d + e'

      > Let [X = d + e', Y = a + bc, Y' = a'(b' + c')]

### Eliminating Terms:

1. Theorem: a'b+a'bc = a'bc

   > [X = a'b]

2. Example: 

   1. a'bc' + bcd + a'bd = a'bc' + bcd

      > [X = c, Y = bd, Z = a'b]

### Eliminating Literals:

1. Theorem: X + X'Y = X + Y

2. Example:

   1. a'b + a'b'c'd' + abcd' 

      = a'(b + b'c'd') + abcd' 

      = a'(b + c'd') + abcd'

      = a'b + a'c'd + abcd' 

      = b(a' + acd') + a'c'd'

      = b(a' + cd' + a'c'd') 

      = a'b + bcd' +a'c'd'

### Adding Redundant:

1. Theorem: adding (X + X'), multiply by (X + X'), adding YZ to XY + X'Z, adding zy to y

2. Example:

   1. WX + XY +X'Z'+ WY'Z'

      = WX + XY + X'Z' + WY'Z' + WZ'

      = WX + XY + X'Z' + WZ'

      = WX + XY = X'Z' = WZ'

      = WX + XY +X'Z'

### Example:

1. a'b'c'd' + a'bc'd' + a'bd + a'bc'd + abcd + acd' + b'cd'

   = a'c'd' + a'bd + abcd + acd' + b'cd'

   = a'c'd' + bd(a' + ac) + acd' + b'cd'

   = a'c'd' + a'bd + bcd + acd' + b'cd'

   = a'c'd' + a'bdbcd + acd' + b'cd' + abc

   = a'c'd' + a'bd + b'cd' + abc

2. (a' + b' + c')(a' + b' + c)(b' + c)(a + c)(a + b + c)

   = (a' + b')(b' + c)(a + c)

   = (a' + b')(a + c)